#  C)

#### Composition
Let $A(x), B(x)$ both be FPS.

We have 


$$\begin{align*}
A(B(x)) &= \sum_{n=0}^{\infty}a_nB(x)^n \\
&= a_0 + a_1B(x) + a_2B(x)^2...\\
&= a_0 + a_1(b_0 + b_1x + b_2x^2) + a_2(b_0 + b_1x + b_2x^2)^2...\\
&= (a_0 + a_1b_0+a_2b_0^2+...)x^0 + ...
\end{align*}$$
We see that the only way for the coefficients to NOT be an infinite sum is to have either:

1. $b_0 = 0$ 
2. $A(x)$ is a polynomial, this way the coefficients are eventually all 0

#### Inverse

Let $A(x)$ be a formal power series, for $A(x)$ to have a multiplicative inverse, there must exist FPS $B(x)$ such that $A(x)B(x) = 1$

	Consider the definition of multiplication of two FPS:

$$\begin{align*}
A(x)B(x) &= \sum^{\infty}_{n=0} (\sum^{n}_{k=0}a_kb_{n-k})x^n \\
&= (a_0b_0)x^0 + (a_0b_1 + a_1b_0)x^1 + (a_0b_2 +a_1b_1 + a_2b_0)x^2...
\end{align*}$$

We see that if we want $A(x)B(x) = 1$, it must be that
$$\begin{align*}
a_0b_0 &= 1 \tag{row 0}\\
a_0b_1 + a_1b_0 &= 0 \tag{row 1}\\
a_0b_2 + a_1b_1 + a_2b_0 &= 0 \tag{row 2}\\
\vdots
\end{align*}$$
We see that for any $k$ row, we can solve for $b_k$ recursively by collecting all the terms which does not contain $c_k$ and divide both sides by $b_0$. Since this is a recursive operation ($b_k$ depends on $b_{k-1}$), we must be able to calculate $b_0$, which means that $b_0 = \frac{1}{a_0}$ , $a_0 \neq 0$ .