---
alias: []
---
# Formal Deduction in Propositional Logic
‚ùå‚úîÔ∏è‚úÖüìó

We have seen how to prove the validity  of arguments by using truth tables and other semantic methods. (tautological consequence, "$\vDash$"). We can use a purely syntactic approach, that is, we give **formal rules of deduction** which are purely **syntactic**
```ad-def
**Formal deducibility:** Denoted $\vdash$, this will allow us to **mechanically/syntactically** check the correctness of a proof that an arugment is valid.

**Complete Definition:** A formula $A$ is **formally deducible** from $\Sigma$, written as $\Sigma \vdash A$, iff $\Sigma \vdash A$ is generated by a finite number of applications of the rules of formal deduction.
```

```ad-note
The intuitive meaning of $\vdash$ is similar to the meaning of $\vDash$, in that it signifies **argument validity**. However, the method of proving validity if very different.

The word "formal" signifies that we will only be concerned with the *syntactic form* of formulas. The proofs themselves will *not refer to any semantic properties*. The correctness of proof can be checked mechanically.
```

Formal deducibility is a relation between a set of formulas $\sum$(called the premises) and a formula $A$ (called the conclusion).

We use the symbol $\vdash$ to denote the relation of formal decuibility and write 
$$\Sigma \vdash A$$
to mean that $A$ is *formally deducible*, or *provable* from $\sum$

For convenience, we will write sets as sequences:
- If $\Sigma = \set {A_1, A_2, A_3,...}$ is a set of formulas, then $\Sigma$ may be written as a sequence, $A_1,A_2,...A_n$
- Since the premises are elements of a set, the order in which the premises in $\Sigma$ *does not matter*
- The set $\Sigma \cup \set A$, where $A$ is a formula, may be writte as $\Sigma, A$
- $\Sigma \cup \Sigma$ may be written as $\Sigma, \Sigma'$

## The 11 rules of formal deduction

For any formulas $A, B, C$, and any set $\Sigma$ of formulas:

| Index, Notation                   | Rule                                                                                                                                     | Name                          |
| --------------------------------- | ---------------------------------------------------------------------------------------------------------------------------------------- | ----------------------------- |
| (1) (Ref)                         | $A \vdash A$ is a theorem                                                                                                                | Reflexivity                   |
| (2) (+)                           | **IF** $\Sigma \vdash A$ is a theorem, <br /> **THEN** $\Sigma, \Sigma' \vdash A$ is a theorem                                                   | Addition of premises          |
| (3) ($\neg \space -$)             | **IF** $\Sigma, \neg A \vdash B$ is a theorem and $\Sigma, \neg A \vdash \neg B$ is a theorem, <br />**THEN** $\Sigma \vdash A$ is a theorem     | Negation elimination          |
| (4) ($\to \space -$)              | **IF** $\Sigma \vdash A \to B$ is a theorem and $\Sigma \vdash A$ is a theorem <br /> **THEN** $\Sigma \vdash B$ is a theorem                    | Implies elimination           |
| (5) ($\to \space +$)              | **IF** $\Sigma, A \vdash B$ is a theorem, <br /> **THEN** $\Sigma \vdash A \to B$ is a theorem                                                   | Implies introduction          |
| (6) ($\land \space -$)            | **IF** $\Sigma \vdash A \land B$ is a theorem, <br /> **THEN**   $\Sigma \vdash A$ is a theorem and $\Sigma \vdash B$ is a theorem.              | AND elimination               |
| (7) ($\land \space +$)            | **IF** $\Sigma \vdash A$ and $\Sigma \vdash B$ is a theorem, <br /> **THEN** $\Sigma \vdash A \land B$ is a theorem                              | AND introduction              |
| (8) ($\lor \space -$)             | **IF** $\Sigma, A \vdash C$ is a theorem and $\Sigma, B \vdash C$ is a theorem, <br /> **THEN** $\Sigma, A \lor B \vdash C$ is a theorem         | OR elimination                |
| (9) ($\lor \space +$)             | **IF** $\Sigma \vdash A$ is a theorem <br />**THEN** $\Sigma \vdash A \lor B$ is a theorem and $\Sigma B \vdash \lor A$ is a theorem               | OR introduction               |
| (10) ($\leftrightarrow \space -$) | **IF** $\Sigma \vdash A \leftrightarrow B$ is a theorem and $\Sigma \vdash A$ is a theorem, <br /> **THEN** $\Sigma \vdash B$ is a theorem       |                               |
| ($\leftrightarrow \space -$)      | **IF** $\Sigma \vdash A \leftrightarrow B$ is a theorem and $\Sigma \vdash A$ is a theorem, <br /> **THEN** $\Sigma \vdash A$ is a theorem       | $\leftrightarrow$ elimination |
| (11) ($\leftrightarrow \space +$) | **IF** $\Sigma, A \vdash B$ is a theorem and $\Sigma, B \vdash A$ is a theorem <br /> **THEN** $\Sigma, \vdash A \leftrightarrow B$ is a theorem | $\leftrightarrow$ introduction     |
|                                   |                                                                                                                                          |                               |

^18c593

(3) prove by contradiction

```ad-note
This 11 rules are everything we accept, everything else must be prove using the 11 rules
```


```ad-example
Prove the following theorem, called "membership rule":

If $A \in \Sigma$
Then $\Sigma \vdash A$

**Proof:**
Suppose $A \in \Sigma$ and $\Sigma' = \Sigma - \set A$ (thus, $\Sigma$ is $A, \Sigma'$)
1. $A \vdash A$ (by Ref)
2. $A, \Sigma' \vdash A$ (by (+),(1))

Step 1 is generated directly by the rule (Ref)
Step 2 is generated by the rule (+), which is then applied to Step (1).
At each step, the rule is applied, and the preceding steps cited  (if any), form a justification for this step, and are written on the right.
These steps constitute a *formal proof* of the last step, $\Sigma \vdash A$
```

```ad-example 
Prove that $A \to B, B \to C \vdash A \to C$.
1. $A \to B, B \to C, A \vdash A \to B$ (by $\in$)
2. $A \to B, B \to C, A \vdash A$ (by $\in$)
3. $A \to B, B \to C, A \vdash B$ (by ($\to \space -$), 1, 2)
4. $A \to B, B \to C, A \vdash B \to C$ (by $\in$)
5. $A \to B, B \to C, A \vdash C$ ($\to \space -$, 4, 3)
6. $A \to B, B \to C \vdash A \to C$ ($\to \space +$, 5)
```
Each step applies either one of the rules of formal deduction, or a theorem which we have already proved

On the right are written justifications for the steps

These six steps form a formal proof of $A \to B, B \to C \vdash A \to C$
```ad-note
We can used previously proved theorems even though the formal rules of deduction do note specify the use of "proved theorems", since we can, instead of invoking a proved theorem, we could insert it's proof.
```

```ad-def 
**Complete Definition:** A formula $A$ is **formally deducible** from $\Sigma$, written as $\Sigma \vdash A$, iff $\Sigma \vdash A$ is generated by a finite number of applications of the rules of formal deduction.
```

^67e85c

## Formal proof
By the above edefinition, $\Sigma \vdash A$ holds IFF there's a finite sequence
$$\begin{gather}
1. \Sigma_1 \vdash A_1 \\
...\\
n. \Sigma_n \vdash A_n
\end{gather}
$$
such that
- each term is generated by one of [[#The 11 rules of formal deduction]]
- $\Sigma_n \vdash A_n$ is $\Sigma \vdash A$, that is , $\Sigma_n = \Sigma$, $A_n = A$

Comments:

- A demonstrated $\Sigma \vdash A$ (that is, for which we have a formal proof) is called a *scheme of formal deduicibility*, or a **theorem**
- Rules of formal deduction are purely **syntactic**
```ad-example
From two (not necessarily consective) "lines" in a proof:
$$\begin{gather}
(i). \Sigma, \neg A \vdash B \\
(ii). \Sigma, \neg A \vdash \neg B
\end{gather}$$

We can generate the new line
$$ (iii). \Sigma \vdash A$$
```
Therefore, it can be checked **mechanically** whether the rules of formal deduction are used correctly.

### Checking a proof
We can check whether a sequence of steps is indeed a [[#Formal proof]] of a "scheme of formal deducibility") (theorem), we:
- Check whether the rules are applied correctly at each steps
- Check whether the last term of the proof is identical with the desired scheme of formal deducibility (theorem)

### Finding a proof
Work in reverse

### Formal deduction proof strategies
- **If the conclusion is an implication**, ex. $\Sigma \vdash A \to B$, then try using implication introduction. Prove $\Sigma, A \vdash B$ first, then apply implies introducction
- **If the premises contain a disjunction**, that is, if we have to prove $\Sigma, A \lor B \vdash C$, we prove seperately $\Sigma, A \vdash C$ (case 1), then $\Sigma, B \vdash C$ (case 2), and put the two proofs together with one apllications of $(\lor -)$
- **If we have to prove $A\to B$** and the direct proof doesn't work, try proving the contrapositive $\neg B \vdash \neg A$. Then use the contrapositive theorem.
 `ris:ErrorWarning` you must prove the theorem first
- **If everything else fails**, try proof by contradiction $(\neg-)$
	- If we want to prove $\Sigma \vdash B$
	- Prove $\Sigma, \neg B \vdash C$ for some formula C (any C is ok!)
	- Prove $\Sigma, \neg B \vdash \neg C$ for the same C
- At the beginning of the proof of a new theorem $\Sigma \vdash A$, the premises do not necessarily have to coincide with $\Sigma$, as long as we end up with the same thing, it's ok!
# Taughtological consequences vs deducibility
- Taughtological consequence belongs to **semantics**, while the latter belongs to **Synxtax**
- **Both are not symbol in $L^p$**

```ad-note
The connection between $\vDash$ and $\to$ is 
$A \vDash B$ iff $A \to B$ is a tautology.

The connection between $\vdash$ and $\to$ is
$A \vdash B$ iff $\emptyset \vdash A \to B$ (exercise)
```

# Proving statement about formal deduction 

We can use structure induction 
Relate: [[]]
